Flow.lean
@@ -1,13 +1,13 @@
-import Flow.Lang.Defs
-import Flow.Lang.CFG
-import Flow.Lang.Eval
+import Flow.TIP.Defs
+import Flow.TIP.CFG
+import Flow.TIP.Eval
 
-import Flow.Eval.Refinement
-import Flow.Eval.Located
-import Flow.Eval.Collection
+import Flow.TIP.Correspondence.Refinement
+import Flow.TIP.Correspondence.Located
+import Flow.TIP.Analyses.CP
+import Flow.TIP.Analyses.Collection
 
 import Flow.Analysis.Lattice
 import Flow.Analysis.Worklist
 import Flow.Analysis.WorklistProofs
 import Flow.Analysis.Generic
-import Flow.Analysis.CP
